cava/Cava/Lib/Retiming.v
@@ -26,77 +26,48 @@ Require Import Cava.Lib.Combinators.
 Require Import Cava.Lib.Multiplexers.
 Import ListNotations Circuit.Notations.
 
-(* Define a restricted type format for the delay circuits to work with *)
-Section WithCava.
-  Context `{semantics : Cava}.
-  (* gives the shape of a collection of signals *)
-  Inductive itype : Type :=
-  | ione (t : SignalType)
-  | ipair (i1 i2 : itype)
-  .
-  Scheme Equality for itype.
-
-  (* gives the Gallina tuple for the collection of signals specified *)
-  Fixpoint ivalue (i : itype) : Type :=
-    match i with
-    | ione t => signal t
-    | ipair a b => ivalue a * ivalue b
-    end.
-
-  Fixpoint idefault (i : itype) : ivalue i :=
-    match i with
-    | ione t => defaultSignal
-    | ipair a b => (idefault a, idefault b)
-    end.
-End WithCava.
-
 Section WithCava.
   Context `{semantics : Cava}.
 
-  (* make a circuit with one delay for each signal, given the delays' reset
-     values *)
-  Fixpoint delays (t : itype) : Circuit (ivalue t) (ivalue t) :=
+  (* make a circuit with one delay for each signal, given reset values *)
+  Fixpoint delays {t : type} : value (signal:=combType) t -> Circuit t t :=
     match t with
-    | ione t => Delay (t:=t)
-    | ipair a b => Par (delays a) (delays b)
+    | tzero => fun _ => Id
+    | tone t => DelayInit
+    | tpair t1 t2 => fun v => Par (delays (fst v)) (delays (snd v))
     end.
 
   (* get the value stored in the 1-delay circuit *)
-  Fixpoint delays_get {t : itype}
-    : circuit_state (delays t) -> ivalue t :=
+  Fixpoint delays_get {t : type}
+    : forall {v : value t}, value (circuit_state (delays v)) -> value t :=
     match t with
-    | ione _ => snd
-    | ipair _ _ => fun st => (delays_get (fst st), delays_get (snd st))
+    | tzero => fun _ _ => tt
+    | tone _ => fun _ => snd
+    | tpair _ _ => fun _ st => (delays_get (fst st), delays_get (snd st))
     end.
 
-  (* make a circuit with repeated delays for each signal, given the delays'
-     reset values for each layer *)
-  Fixpoint ndelays (n : nat) (t : itype) : Circuit (ivalue t) (ivalue t) :=
-    match n with
-    | 0 => Id
-    | S m => ndelays m t >==> delays t
+  (* make a circuit with repeated delays for each signal *)
+  Fixpoint ndelays {t : type} (v : list (value (signal:=combType) t)) : Circuit t t :=
+    match v with
+    | [] => Id
+    | v0 :: v => ndelays v >==> delays v0
     end.
 
   (* get all the values stored in the n-delay circuit *)
-  Fixpoint ndelays_get {n t} : circuit_state (ndelays n t) -> list (ivalue t) :=
-    match n with
-    | 0 => fun _ => []
-    | S _ => fun st => delays_get (snd st) :: ndelays_get (fst st)
+  Fixpoint ndelays_get {t v} : value (circuit_state (@ndelays t v)) -> list (value t) :=
+    match v with
+    | [] => fun _ => []
+    | _ :: _ => fun st => delays_get (snd st) :: ndelays_get (fst st)
     end.
+
 End WithCava.
 
-(* it's possible to define is_delays directly without using itype, but then
-   inversion can't handle the type mismatches if the types are not just plain
-   identifiers, and you get nonsensical cases where e.g. unit = t1 * t2 *)
-Inductive is_delays' : forall t, Circuit (ivalue t) (ivalue t) -> Prop :=
-| is_delays'_delay : forall t resetval, is_delays' (ione t) (DelayInit (t:=t) resetval)
-| is_delays'_par :
-    forall t1 t2 c1 c2,
-      is_delays' t1 c1 -> is_delays' t2 c2 ->
-      is_delays' (ipair t1 t2) (Par c1 c2)
-.
 Inductive is_delays : forall {t}, Circuit t t -> Prop :=
-| is_delays_is_delays' : forall t c, is_delays' t c -> is_delays c
+| is_delays_delay : forall t resetval, is_delays (DelayInit (t:=t) resetval)
+| is_delays_par :
+    forall t1 t2 c1 c2,
+      is_delays c1 -> is_delays c2 ->
+      @is_delays (t1 * t2) (Par c1 c2)
 .
 
 Inductive is_ndelays : forall {t}, nat -> Circuit t t -> Prop :=
@@ -112,69 +83,66 @@ Definition retimed {i o} (n : nat) (c1 c2 : Circuit i o) : Prop :=
     is_ndelays n delay_circuit
     /\ cequiv c1 (delay_circuit >==> c2).
 
-Definition mealy {i o} (c : Circuit i o)
-  : Circuit (i * circuit_state c) (o * circuit_state c) :=
-  Comb (fun '(input, st) =>
-          let st_out := step c st input in
-          (snd st_out, fst st_out)).
-
-(* we don't really want *full* mealy; just for loops -- and this state can be itype!! *)
-
-Fixpoint loops_state {i o} (c : Circuit i o) : itype :=
+Fixpoint loops_state {i o} (c : Circuit i o) : type :=
   match c with
-  | Comb _ => ione Void
+  | Comb _ => tzero
   | First f => loops_state f
   | Second f => loops_state f
-  | Compose f g => ipair (loops_state f) (loops_state g)
-  | @DelayInitCE _ _ t _ => ione Void
-  | @LoopInitCE _ _ _ _ t _ body => ipair (loops_state body) (ione t)
+  | Compose f g => loops_state f * loops_state g
+  | @DelayInitCE _ _ t _ => tzero
+  | @LoopInitCE _ _ _ _ t _ body => loops_state body * t
   end.
+
+Fixpoint loops_reset_state {i o} (c : Circuit i o)
+  : value (signal:=combType) (loops_state c) :=
+  match c with
+  | Comb _ => tt
+  | First f => loops_reset_state f
+  | Second f => loops_reset_state f
+  | Compose f g => (loops_reset_state f, loops_reset_state g)
+  | DelayInitCE _=> tt
+  | LoopInitCE resetval body => (loops_reset_state body, resetval)
+  end.
+
 Require Import ExtLib.Structures.Monad.
 Import MonadNotation.
 
 (* Pull the loops out of the circuit completely *)
-(* TODO: ask Ben B to remind me whose idea this was so they can be credited here *)
 Fixpoint loopless {i o} (c : Circuit i o)
-  : Circuit (i * ivalue (loops_state c)) (o * ivalue (loops_state c)) :=
+  : Circuit (i * loops_state c) (o * loops_state c) :=
   match c as c in Circuit i o
-        return Circuit (i * ivalue (loops_state c))
-                       (o * ivalue (loops_state c)) with
+        return Circuit (i * loops_state c) (o * loops_state c) with
   | Comb f => First (Comb f)
   | First f =>
-    Comb (fun '(x1,x2,st) => ret (x1,st,x2)) (* rearrange *)
+    Comb (i:=(_*_*_)) (fun '(x1,x2,st) => ret (x1,st,x2)) (* rearrange *)
          >==> First (loopless f) (* recursive call *)
-         >==> Comb (fun '(y1,st,y2) => ret (y1,y2,st)) (* rearrange *)
+         >==> Comb (i:=(_*_*_)) (fun '(y1,st,y2) => ret (y1,y2,st)) (* rearrange *)
   | Second f =>
-    Comb (fun '(x1,x2,st) => ret (x1,(x2,st))) (* rearrange *)
+    Comb (i:=(_*_*_)) (fun '(x1,x2,st) => ret (x1,(x2,st))) (* rearrange *)
          >==> Second (loopless f) (* recursive call *)
-         >==> Comb (fun '(y1,(y2,st)) => ret (y1,y2,st)) (* rearrange *)
+         >==> Comb (i:=(_*(_*_))) (fun '(y1,(y2,st)) => ret (y1,y2,st)) (* rearrange *)
   | Compose f g =>
-    Comb (fun '(x,(st1,st2)) => ret (x,st1,st2)) (* rearrange *)
+    Comb (i:=(_*(_*_))) (fun '(x,(st1,st2)) => ret (x,st1,st2)) (* rearrange *)
          >==> First (loopless f) (* recursive call *)
-         >==> Comb (fun '(y,st1,st2) => ret (y,st2,st1)) (* rearrange *)
+         >==> Comb (i:=(_*_*_)) (fun '(y,st1,st2) => ret (y,st2,st1)) (* rearrange *)
          >==> First (loopless g) (* recursive call *)
-         >==> Comb (fun '(z,st2,st1) => ret (z,(st1,st2))) (* rearrange *)
+         >==> Comb (i:=(_*_*_))  (fun '(z,st2,st1) => ret (z,(st1,st2))) (* rearrange *)
   | DelayInitCE resetval => First (DelayInitCE resetval)
-  | LoopInitCE resetval body =>
-    (* need : i * Bit * (lstate body * t) -> o * (lstate body * t) *)
-    (* loopless body : i * t * lstate body -> o * t * lstate body *)
-    Comb (fun '(x,en,(body_st, loop_st)) =>
-            ret (en,loop_st,(x,loop_st,body_st))) (* rearrange *)
+  | @LoopInitCE _ _ _ _ s resetval body =>
+    (Comb (i:=(_*_*(_*_)))
+          (fun '(x,en,(body_st, loop_st)) =>
+             ret (en,loop_st,(x,loop_st,body_st)))) (* rearrange *)
          >==> Second (loopless body) (* recursive call *)
-         >==> Comb (fun '(en, loop_st, (y, loop_st', body_st')) =>
-                      loop_st' <- mux2 en (loop_st,loop_st') ;;
-                      (y,(body_st',loop_st')))
+         >==> (Comb (i:=(Bit * _ * (_ * _ * _))) (o:=(_*(_* _)))
+                    (fun '(en, loop_st, (y, loop_st', body_st')) =>
+                       loop_st' <- mux2 en (loop_st,loop_st') ;;
+                       ret (y,(body_st',loop_st'))))
   end.
 
-
-(* can make a def that re-adds loops only to outside, then prove all circuits
-   equivalent to this transformation *)
-
 Definition phase_retimed {i o} (n m : nat) (c1 c2 : Circuit i o) : Prop :=
-  exists state_delays input_delays
-    (proj : ivalue (loops_state c1) -> ivalue (loops_state c2)),
-    is_ndelays n state_delays
-    /\ is_ndelays m input_delays
-    /\ cequiv (loopless c1 >==> Second (Comb (fun st => ret (proj st))))
-             (Par input_delays (Comb (fun st => ret (proj st)) >==> state_delays)
-                  >==> loopless c2).
+  exists state_resets input_resets,
+    length state_resets = n
+    /\ length input_resets = m
+    /\ cequiv c1 (LoopInit (loops_reset_state c2)
+                          (Par (ndelays input_resets) (ndelays state_resets)
+                           >==> loopless c2)).
